\DiaryEntry{Generating Functions, Part 5}{2015-09-25}{GenFuncs}

This post provides several examples regarding sequence shifts and initial conditions.

\subsection{First-order Example}\label{first-order-example}

\subsubsection{Left-Shift}\label{left-shift}

Consider the recurrence relation

\[a_{n} = 2a_{n-1}, \quad a_0 = 1\]

from which we obtain obtain the generating function and its series expansion

\[ A(z) = 2zA(z) + 1 \rightarrow A(z) = \frac{1}{1-2z} = 1 + 2z + 4z^2 + 8z^3 + \cdots\]

\subsubsection{Right-Shift}\label{right-shift}

We can also express the recurrence relation as follows

\[a_{n+1} = 2a_n, \quad a_0 = 1\]

from wihch we obtain

\[ \frac{A(z) - 1}{z} = 2A(z) \rightarrow A(z) = \frac{1}{1-2z} = 1 + 2z + 4z^2 + 8z^3 + \cdots\]

which is the same.

\subsection{Fibonacci Sequences (Second-order
Example)}\label{fibonacci-sequences-second-order-example}

\subsubsection{Left-Shift}\label{left-shift-1}

Consider the sequence described by

\[ a_n = a_{n-1} + a_{n-2}, \quad a_0 = 0, a_1 = 1 \]

For the generating function, we have

\[ A(z) = z A(z) + z^2 A(z) + z \rightarrow A(z) = \frac{z}{1-z-z^2} = z + z^2 + 2z^3 + 3z^4 + \cdots \]

When dealing with left-shifts only an initial condition for $a_1$ is allowed in case of second-order relations. As an example for a recurrence relation which violates this condition, consider the same recurrence relation but with different initial conditions

\[ a_n = a_{n-1} + a_{n-2}, \quad a_0 = 1, a_1 = 1 \]

We obtain

\[ A(z) = z A(z) + z^2 A(z) + z + 1 \rightarrow A(z) = \frac{1 + z}{1-z-z^2} = 1 + 2z + 3z^2 + 5z^3 + \cdots \]

This sequence fulfills the recurrence relation but \textbf{violates the initial conditions}.

\subsubsection{Right-Shift}\label{right-shift-1}

In case of right-shifts, arbitrary initial conditions can be specified. Reformulating the last example we obtain

\[ a_{n+2} = a_{n+1} + a_{n}, \quad a_0 = 1, a_1 = 1 \]

and for the generating function

\[ \frac{A(z) - 1 - z}{z^2}  = \frac{A(z) - 1}{z} + A(z) \rightarrow A(z) = \frac{1}{1-z-z^2} = 1 + z + 2z^2 + 3z^3 + 5z^4 + \cdots \]

\subsection{Third-order Example}\label{third-order-example}

\subsubsection{Left-Shift}\label{left-shift-2}

Consider the following example

\[ a_n = a_{n-1} + a_{n-2} + a_{n-3}, \quad a_0 = 0, a_1 = 1, a_2 = 1 \]

wich violates the condition on the inital values stated above $a_1 \neq 0$. We have

\[ A(z) = zA(z) + z^2A(z) + z^3 A(z) + z + z^2 \rightarrow A(z) = \frac{z + z^2}{1 - z - z^2 - z^3} = z + 2z^2 + 3z^3 + 6z^4 + 11z^5 + 20 z^6 + \cdots\]

which fulfills the recurrence relation but again, the sequence \textbf{violates the initial conditions}.

Next we consider an example which fulfills the condition on the inital values: We have

\[ a_n = a_{n-1} + a_{n-2} + a_{n-3}, \quad a_0 = 0, a_1 = 0, a_2 = 1 \]

and obtain

\[ A(z) = zA(z) + z^2A(z) + z^3 A(z) + z^2 \rightarrow A(z) = \frac{z^2}{1 - z - z^2 - z^3} = z^2 + z^3 + 2z^4 + 4z^5 + 7 z^6 + \cdots\]

which is correct.

\subsubsection{Right-Shift}\label{right-shift-2}

Again, this approach is easier and more flexible. Reformulating the example from above, we have

\[ a_{n+3} = a_{n+2} + a_{n+1} + a_{n}, \quad a_0 = 0, a_1 = 1, a_2 = 1 \]

For the generating function we obtain

\[ \frac{A(z) - z - z^2}{z^3}  = \frac{A(z) - z}{z^2} + \frac{A(z) - 0}{z} + A(z) \rightarrow A(z) = \frac{z}{1-z-z^2-z^3} = z + z^2 + 2z^3 + 4z^4 + 7z^5 + 13z^6 + \cdots \]

This approach allows \textbf{any} initial conditions; for example

\[ a_{n+3} = a_{n+2} + a_{n+1} + a_{n}, \quad a_0 = 1, a_1 = 2, a_2 = 3 \]

gives

\[ \frac{A(z) - 1 - 2z - 3z^2}{z^3}  = \frac{A(z) - 1 - 2z}{z^2} + \frac{A(z) - 1}{z} + A(z) \rightarrow A(z) = \frac{1 + z}{1-z-z^2-z^3} = 1 + 2z + 3z^2 + 6z^3 + 11z^4 + \cdots \]

\subsection{SymPy Solutions}\label{sympy-solutions}

Calculating generating functions and performing series expansions like in the examples is tedious; SymPy can help:

\begin{verbatim}
import sympy as sym

x, y, n, a = sym.symbols("x y n a")

# solve for generating function
F = sym.solve((a-1-2*x-3*x**2)/x**3 - (a-1-2*x)/x**2 - (a-1)/x - a, a)
F = F[0]

res = sym.series(F, x, 0, 10)
sym.pprint(res)

           2     3      4      5      6      7       8       9
1 + 2x + 3x  + 6x  + 11x  + 20x  + 37x  + 68x  + 125x  + 230x  + ...
\end{verbatim}
