\DiaryEntry{Interesting Sums, III}{2016-05-21}{Maths}

\subsection{Sums with a factorial}

The exponential function \(\exp(x)\) has the following Taylor series
expansion:

\[
\exp(x) = \sum_{n=0}^\infty \frac{x^n}{n!}
\]

Taking derivatives with respect to \(x\) on both sides yields

\[
\exp(x) = \sum_{n=1}^\infty \frac{n x^{n-1}}{n!} = \sum_{n=1}^\infty \frac{x^{n-1}}{(n-1)!} = \sum_{n=0}^\infty \frac{x^n}{n!}
\]

Ok, this is not so interesting (especially as the LHS stays the same).

Let's try this

\[
\sum_{n=0}^\infty \frac{x^{n+1}}{n!} = \sum x \frac{x^n}{n!} = x \sum \frac{x^n}{n!} = x e^x
\]

Taking the derivative with respect to \(x\) yields

\[
e^x (1+x) = \sum_{n=0}^\infty \frac{(n+1)x^n}{n!}
\]

Considering \(x=1\), we obtain

\[
\sum_{n=0}^\infty \frac{(n+1)}{n!} = 2e
\]

We can differentiate another time and get

\[
e^x (2+x) = \sum_{n=0}^\infty \frac{n(n+1)x^{n-1}}{n!}
\]

which evaluates to

\[
\sum_{n=0}^\infty \frac{n(n+1)}{n!} = 3e
\]

at \(x=1\). Ladies and Gentlemen, I think we have a pattern here :-).
Start with

\[
\frac{d}{dx}xe^x = xe^x + e^x
\]

and

\[
\frac{d^2}{dx^2}xe^x = xe^x + e^x + e^x = xe^x + 2e^x
\]

and in general

\[
\frac{d^n}{dx^n}x e^x = xe^x + ne^x
\]

Evaluating this at \(x=1\) yields

\[
\left. \frac{d^n}{dx^n}x e^x \right|_{x=1} = (n+1)e
\]

and from this we obtain the sum

\[
\sum_{n} \frac{(n+1)^{\underline{m}}}{n!} = (m+1)e
\]

where \(x^{\underline{n}} = x(x-1)\cdots(x-n+1)\) is the falling
factorial.
