\DiaryEntry{AM-GM Inequality}{2016-02-02}{Maths}

Proof that

\[
(a_1 \cdots a_n)^{1/n} \leq \frac{a_1 + \cdots + a_n}{n}
\]

For \(n=2\) this is easy: We have
\((x-y)^2 = x^2 + y^2 - 2xy \geq 0 \rightarrow \frac{x^2 + y^2}{2} \geq xy\).
If we replace \(x\) with \(\sqrt{x}\) and \(y\) with \(\sqrt{y}\), we
arrive at

\[
\frac{x + y}{2} \geq \sqrt{xy}
\]

For \(n=4\), we apply the inequality for \(n=2\) two times: The first
time to \((a_1 a_2)^{1/2}\) and \((a_3 a_4)^{1/2}\):

\[
(a_1 a_2 a_3 a_4)^{1/4} = \left( (a_1 a_2)^{1/2}(a_3 a_4)^{1/2} \right)^{1/2} \leq \frac{(a_1 a_2)^{1/2} + (a_3 a_4)^{1/2}}{2}
\]

Applying the inequality a second time to we arrive at

\[
(a_1 a_2 a_3 a_4)^{1/4} \leq \frac{1}{2} \frac{a_1 + a_2}{2} + \frac{1}{2} \frac{a_3 + a_4}{2} = \frac{a_1 a_2 a_3 a_4}{4}
\]

By repeatedly applying this inequality, we can extend to cases
\(n = 2^k\):

\begin{equation}
\label{eq:amgm2k}
(a_1 a_2 \cdots a_{2^k})^{1/2^k} \leq \frac{a_1 + \cdots + a_{2^k}}{2^k}
\end{equation}

The question is how to proof the inequality for general \(n\). To this
end we take an \(n < 2^k\) and define a sequence \(\alpha_i\) as
follows:

\[
\alpha_i = \begin{cases}
a_i & \mbox{if } i \leq n \\
A & \mbox{if } i > n \end{cases}
\]

where \(A = \frac{a_1 + \cdots + a_n}{n}\). In other words, we simply
pad the original sequence \(a_i\) with the arithmetic average \(A\) to
give a length-\(2^k\) sequence. The average \(A\) is contained
\(2^k - n\) times in the sequence \(\alpha_i\) and therefore equation
\eqref{eq:amgm2k} yields

\[
(a_1 a_2 \cdots a_n A^{2^k - n})^{1/2^k} \leq \frac{a_1 + \cdots + a_n + (2^k - n) A}{2^k} = \frac{nA + 2^k A - nA}{2^k} = A
\]

We can move the \(A\) term to the right side as follows:

\[
(a_1 a_2 \cdots a_n)^{1/2^k} A^{(2^k - n)\frac{1}{2^k}} = (a_1 a_2 \cdots a_n)^{1/2^k} A^{1 - \frac{n}{2^k}} \leq A \rightarrow (a_1 a_2 \cdots a_n)^{1/2^k} \leq A^{1 - (1 - \frac{n}{2^k})} = A^{\frac{n}{2^k}}
\]

Raising both sides to \(2^k / n\), we finally obtain the AM-GM
inequality

\[
(a_1 a_2 \cdots a_n)^{1/n} \leq A = \frac{a_1 + \cdots + a_n}{n}
\]
