\DiaryEntry{Möbius Transform, I}{2017-12-22}{Maths}

Based on Visual Complex Analysis. The Möbius Transform is defined as

\bee
H(z) = \frac{az+b}{cz+d}
\eee

and the book claims that this can be interpreted as a sequence of the following transformations

\begin{align*}
z & \rightarrow z + d/c \\
z & \rightarrow 1/z \\
z & \rightarrow - \frac{ad-bc}{c^2} z \\
z & \rightarrow z + a/c
\end{align*}

Let's show that this is correct: Combining the first two tranformations into $f(z)$ yields

\bee
f(z) = \frac{1}{z + \frac{d}{c}},
\eee

combining this with the third yields

\bee
g(z) = - \frac{ad-bc}{c^2} \frac{1}{z + \frac{d}{c}}
\eee

and combining with the fourth, we obtain the final result

\bee
h(z) = - \frac{ad-bc}{c^2} \frac{1}{z + \frac{d}{c}} + \frac{a}{c}
\eee

Now we can start simplifying as follows

\begin{align*}
h(z) & = \frac{bc-ad}{c^2} \frac{c}{cz + d} + \frac{a}{c} = \frac{bc-ad}{c} \frac{1}{cz + d} + \frac{a}{c} = \frac{bc-ad}{c(cz+d)} + \frac{a}{c} 
\\ & = \frac{bc-ad+a(cz+d)}{c(cz+d)} = \frac{bc-ad+acz+ad}{c(cz+d)} = \frac{az+b}{cz+d}
\end{align*}
\qed
