\DiaryEntry{Interesting Integrals, Part 5}{2017-02-06}{Integrals}

\subsection{Task}

We want to solve the following integral

\bee
\int x^2 e^x dx
\eee

The ``Standard-approach'' is to use integration by parts (two times) and wade through the mess. In the following, we present a simpler solution.

\subsection{Simpler Way}

Consider the function

\be\label{2017-02-06:def}
f(t) = \int e^{tx} dx = \frac{1}{t} e^{tx}
\ee
%
Differentiating the integral with respect to $t$ yields

\bee
f'(t) = \int x e^{tx} dx, f''(t) = \int x^2 e^{tx} dx
\eee
%
At the value $t=1$, we then have

\bee
f''(1) = \int x^2 e^x dx
\eee
%
In \eqref{2017-02-06:def}, we now need to differentiate the righthand side ($\frac{1}{t} e^{tx}$) two times. We have

\bee
\frac{d}{dt} \frac{1}{t} e^{tx} = \frac{1}{t} x e^{tx} - \frac{1}{t^2} e^{tx}
\eee
%
and

\bee
\frac{d^2}{dt^2} \frac{1}{t} e^{tx} = -\frac{1}{t^2}x e^{tx} + \frac{1}{t}x^2 e^{tx} + \frac{2}{t^3} e^{tx} - \frac{1}{t^2}x e^{tx}
\eee
%
We are almost done; we now need to consider the 2nd derivative at $t=1$ in order to obtain
%
\bee
f''(1) = \int x^2 e^x dx = -x e^x + x^2 e^x 2 e^x -x e^x = e^x(x^2 - 2x + 2) \qed
\eee
%
This result can be checked with e.g. SymPy or Wolfram Alpha.

\begin{verbatim}
import sympy as sym
from sympy.abc import x,t

fint = 1/t*sym.exp(t*x)

dfn = fint.diff(t,2)
sym.pprint(dfn.subs(t,1))

sym.pprint(sym.integrate(x**2 * sym.exp(x), x))

\end{verbatim}

\subsection{Generalization}

Of course it is possible to consider higher-order derivatives; we have

\bee
f^{(n)}(1) = \int x^n e^{xt} dx
\eee
%
and need to calculate the n-th derivative
%
\bee
\frac{d^n}{dt^n} \frac{1}{t} e^{tx} = \ldots
\eee
%
These tedious tasks can e.g. be done with SymPy:

\begin{verbatim}
import sympy as sym
from sympy.abc import x,t

N = 4

fint = 1/t*sym.exp(t*x)

dfn = fint.diff(t,N)
sym.pprint(dfn.subs(t,1))

sym.pprint(sym.integrate(x**N * sym.exp(x), x))

\end{verbatim}
