\DiaryEntry{Inside Interesting Integrals, 7 (Section 2.5)}{2018-03-26}{Integrals}

\subsection{Challenge problem C2.2}

The problem asks for the integral

\bee
\int_0^1 \frac{dx}{x^3+1}
\eee

We first make a partial fraction expansion as follows

\begin{align*}
\int_0^1 \frac{dx}{x^3+1} &= \int_0^1 \frac{1}{3}\frac{1}{x+1} - \frac{1}{3}\frac{x-2}{x^2-x+1} dx \\ &= \int_0^1 \frac{1}{3}\frac{1}{x+1} - \int_0^1 \frac{1}{3} \left[ \frac{1}{2} \frac{2x-1}{x^2-x+1} - \frac{3}{2} \frac{1}{x^2-x+1} \right] dx = I_1 + I_2 + I_3
\end{align*}

where in the second step we split the terms and sneaked in factors so that the enumerator is the derivative of the denominator: $(x^2 - x+1)' = 2x-1$. IN the following, we solve one of the three integrals.

\paragraph{Integral $I_1$:} We set $u=x+1$ and obtain

\bee
\int_0^1 \frac{1}{3}\frac{1}{u} du = \frac{1}{3} \left. \ln (x+1) \right|_0^1 = \frac{1}{3} \ln 2
\eee

\paragraph{Integral $I_2$:} Here we make the substitution $u = x^2-x+1, du/dx = 2x-1, du/(2x-1) = dx$ and arrive at

\bee
\int \frac{2x-1}{x^2-x+1} dx = \int \frac{2x-1}{u} \frac{du}{2x-1} = \ln u = \left. \ln(x^2-x+1) \right|_0^1 = \ln 1 - \ln 1 = 0
\eee

Therefore $I-2 = 0$.

\paragraph{Integral $I_3$:} This integral is solved by completing the square:

\bee
\int \frac{dx}{x^2-x+1} = \int \frac{dx}{x^2-x+\frac{1}{4} + \frac{3}{4}} = \int \frac{dx}{\left(x-\frac{1}{2}\right)^2 + \frac{3}{4}} = \int \frac{dx}{u^2 + \frac{3}{4}}
\eee

where we have set $u=x-1/2$ (and $du/dx=1$). This integral can be solved and we obtain

\begin{align*}
I_3 = \frac{1}{2} \frac{2 \arctan \frac{2u}{\sqrt{3}}}{\sqrt{3}} = \left. \frac{ \arctan \frac{2(x-1/2)}{\sqrt{3}}}{\sqrt{3}} \right|_0^1 & = \frac{\arctan 1/\sqrt{3}}{\sqrt{3}} - \frac{\arctan \left(-1/\sqrt{3}\right) }{\sqrt{3}} \\ & = 2 \arctan \left(1/\sqrt{3}\right)/\sqrt{3} = \frac{\pi}{\sqrt{27}}
\end{align*}

Combining everything together, we arrive at

\bee
\boxed{
\int_0^1 \frac{dx}{x^3+1} = \frac{1}{3} \ln 2 + \frac{\pi}{\sqrt{27}}
}
\eee

We can do this in Maxima as well

\begin{verbatim}
(%i1)	integrate(1/(x^3+1), x, 0, 1);
(%o1)	(6*log(2)+sqrt(3)*%pi)/18+%pi/(2*3^(3/2))
(%i2)	float((6*log(2)+sqrt(3)*%pi)/18+%pi/(2*3^(3/2))), numer;
(%o2)	0.8356488482647211
(%i3)	partfrac(1/(x^3+1), x);
(%o3)	1/(3*(x+1))-(x-2)/(3*(x^2-x+1))
(%i4)	atan(1/sqrt(3));
(%o4)	%pi/6
(%i5)	float(log(2)/3+%pi/3^(3/2)), numer;
(%o5)	0.8356488482647211
\end{verbatim}


\subsection{Challenge problem  C2.3}

Start with the following integral from p. 58 

\be\label{2018-03-26:eq1}
I = \int_0^\infty \frac{dx}{x^4 + 2x^2 \cos(2\alpha) + 1}
\ee

Substitute $y=1/x, dy/dx = -1/x^2, dx = -x^2 dy = -1/y^2 dy$ and we obtain

\bee
I = - \int_\infty^0 \frac{\frac{1}{y^2} dy}{\frac{1}{y^4} + 2\frac{1}{y^2} \cos(2\alpha) + 1} = \int_0^\infty \frac{y^2 dy}{1 + 2y^2 \cos(2\alpha) + 1}
\eee

In the last expression, we can (of course) replace $y$ with $x$ (it's just the integration variable after all) and add it to the original \eqref{2018-03-26:eq1} in order to obtain

\bee
2I = \int_0^\infty \frac{1 + x^2}{x^4 + 2x^2 \cos(2\alpha) + 1} dx
\eee

With the integrand being even, we have

\bee
I = \frac{1}{4} \int_{-\infty}^\infty \frac{1 + x^2}{x^4 + 2x^2 \cos(2\alpha) + 1} dx
\eee

We have $\cos(2\alpha) = 1 - 2 \sin^2(\alpha)$, we can expand the denominator as follows

\bee
x^4 + 2x^2 \cos(2\alpha) + 1 = [x^2 - 2x\sin(\alpha)+1][x^2 + 2x\sin(\alpha)+1]
\eee

and we arrive at

\bee
I = \frac{1}{4} \int_{-\infty}^\infty \frac{1 + x^2}{[x^2 - 2x\sin(\alpha)+1][x^2 + 2x\sin(\alpha)+1]} dx
\eee

Since the integrand is even, we can include an odd function in the numerator without changing the integral value. We choose to include $2x\sin(\alpha)$ and arrive at

\bee
I = \frac{1}{4} \int_{-\infty}^\infty \frac{1 - 2x\sin(\alpha) + x^2}{[x^2 - 2x\sin(\alpha)+1][x^2 + 2x\sin(\alpha)+1]} dx = \frac{1}{4} \int_{-\infty}^\infty \frac{dx}{x^2 + 2x\sin(\alpha)+1}
\eee

We try to complete the square in the denominator; to this end we expand $1 = \sin^2 (\alpha) + \cos^2(\alpha)$ and obtain

\bee
I = \frac{1}{4} \int_{-\infty}^\infty \frac{dx}{x^2 + 2x\sin(\alpha)+ \sin^2 (\alpha) + \cos^2(\alpha)} = \frac{1}{4} \int_{-\infty}^\infty \frac{dx}{[x + \sin(\alpha)]^2 + \cos^2(\alpha)}
\eee

Now we can substitute $u = x+\sin(\alpha)$ (with $du = dx$) and arrive at

\bee
I = \frac{1}{4} \int_{-\infty}^\infty \frac{dx}{u^2 + \cos^2(\alpha)} = \frac{1}{4} \left( \frac{1}{\cos(\alpha)} \right) \arctan\left( \frac{u}{\cos(\alpha)} \right)\bigg|_{-\infty}^\infty = \frac{\pi}{4 \cos(\alpha)} \qed
\eee


\subsubsection{Partial Integration}

We start with the differentiation rule for the product of two functions:

\bee
\left(u(x)v(x)\right)' = u'(x)v(x) + u(x)v'(x)
\eee

If we integrate both sides and rearrange terms, we arrive at

\be
\label{2018-03-26:eq2}
\int u'(x)v(x) dx  = u(x)v(x) - \int u(x)v'(x) dx
\ee

Hidden in the simple-looking formula is the fact that we need to integrate $u'$ in order to arrive at $u$ on the right side. The "trick" is to choose $u$ and $v$ on the LHS in such a way, that (i) integrating $u'$ is possible and (ii) that the integral $\int u(x)v'(x) dx$ is simpler than the original integral.

We can demonstrate this with a very simple example; namely $\int x^3 dx$. We choose $u'=x \rightarrow u=x^2 / 2$ and $v=x^2 \rightarrow v'=2x$. Inserting into above expression, we obtain

\bee
\int x^3 dx = \frac{x^2}{2} x^2 - \int \frac{x^2}{2} 2x dx = \frac{x^4}{2} - \int x^3 dx = \frac{x^4}{2} - \frac{x^4}{4} = \frac{x^4}{4} \qed
\eee

We can do the same trick also with definite integrals like this

\be
\label{2018-03-26:eq3}
\int_A^B u'(x)v(x) dx  = u(x)v(x) \bigg|_A^B - \int_A^B u(x)v'(x) dx
\ee

In the first term on the RHS $u(x)v(x) \bigg|_A^B$, we can exchange the calculation at $A$ and $B$ with multiplication; i.e. we can also write

\bee
\int_A^B u'(x)v(x) dx  = u(x) \bigg|_A^B v(x) \bigg|_A^B - \int_A^B u(x)v'(x) dx
\eee

meaning that we only need to know the definite integral $\int_A^B u'(x)dx$. However, \emph{I think} this is not possible in the second term: Here we need to know $u(x)$, multiply this expression with $v(x)$ and perform the integration \emph{afterwards}. In other words,

\bee
\int_A^B u(x)v'(x) dx \neq \int_A^B \left( \int_A^B u(x)dx \right) v'(x) dx = \int_A^B u(x)dx \cdot \int_A^B v'(x) dx
\eee

where we have realized that $\int_A^B u(x)dx$ is a constant factor and have it moved in front of the outer integral. This makes it pretty obvious why the two expressions cannot be equal.

We can illustrate this with a simple example

\bee
\int_0^1 x \cdot x^2 dx = \frac{x^3}{3}\bigg|_0^1 = \frac{1}{3}
\eee

whereas

\bee
\int_0^1 \left( \int_0^1 x dx \right) x^2 dx = \int_0^1 \left( \frac{x^2}{2} \bigg|_0^1 \right) x^2 dx = \frac{1}{2} \cdot \int_0^1  x^2 dx = \frac{1}{2} \frac{1}{3} = \frac{1}{6} \qed
\eee

We can demonstrate \eqref{2018-03-26:eq2} with a simple example: $\int_0^1 x^3 dx = 1/4$. Setting $u'=x \rightarrow u=x^2 / 2$ and $\int_0^1 u' dx = 1/2$ and $v=x^2 \rightarrow v'=2x$ we have

\bee
\int_0^1 x^3 dx = \frac{1}{2} \cdot x^2 \bigg|_0^1 - \int_0^1 \frac{x^2}{2} 2x dx = \frac{1}{2} - \frac{x^4}{4}\bigg|_0^1 = \frac{1}{2} - \frac{1}{4} = \frac{1}{4} \qed
\eee

\subsubsection{Partial Integration - Examples}

A very simple integral is

\bee
\int x \sin(x) dx
\eee

Here we choose $u$ and $v$ so, that $v'$ is simpler: $u'=\sin(x) \rightarrow u = -\cos(x)$ and $v=x \rightarrow v'=1$. Then we have

\bee
\int x \sin(x) dx = -x \cos(x) + \int \cos(x) dx = \sin(x) - x \cos(x) \qed
\eee

In a similar spirit, we obtain

\bee
\int x e^x dx = xe^x - \int e^x dx = e^x(x-1) \qed
\eee

with $u'=e^x \rightarrow u=e^x$ and $v=x \rightarrow v'=1$.

There is one clever trick, the "unity trick" which can be helpful. In the integral

\bee
\int \ln(x) dx
\eee

set $u'=1 \rightarrow u = x$ and $v = \ln(x) \rightarrow v' = 1/x$. Then we obtain

\bee
\int \ln(x) dx = x \ln(x) - \int x \frac{1}{x} dx = x \ln(x) - x \qed
\eee

A slightly more complicated example is

\bee
I = \int \frac{\ln(x)}{x^2}dx
\eee

Setting $u'=1/x^2 \rightarrow u=-1/x$ and $v=\ln(x) \rightarrow v'=1/x$. Then we have

\bee
I = -\frac{\ln(x)}{x} - \int \left(-\frac{1}{x}\right)\frac{1}{x}dx = -\frac{\ln(x)}{x} + \int \frac{1}{x^2}dx = -\frac{\ln(x)}{x} - -\frac{1}{x} = -\frac{\ln(x)+1}{x} \qed
\eee

Now back to the challenge problem C2.3. We want to show

\bee
\int_0^\infty \frac{dx}{(1+x^4)^{m+1}} = \frac{4m-1}{4m}\int_0^\infty \frac{dx}{(1+x^4)^m}
\eee

Start with

\bee
I = \int_0^\infty \frac{dx}{(1+x^4)^{m}}
\eee

There are three strategies:

\begin{itemize}
	\item Set
	\bee
	u' = \frac{1}{x^4+1}, v = \frac{1}{(x^4+1)^{m-1}}
	\eee
	
	Then we need to find the integral $\int udx$ which is complicated. 
	
	\item Reverse the role of $u$ and $v$ and set 
	\bee
	u' = \frac{1}{(x^4+1)^{m-1}}, v = \frac{1}{x^4+1}
	\eee
	
	where the integral $\int u dx$ is even more complicated.
	
	\item Use the "unity trick" and set
	\bee
	u' = 1, v = \frac{1}{(x^4+1)^m}
	\eee
\end{itemize}

It is actually the last approach which works. In this case $u=x$ and $v' = (-m) 4x^3 (x^4+1)^{-m-1}$ and we obtain

\bee
I = \frac{x}{(x^4+1)^m}\bigg|_0^\infty - \int_0^\infty  (-m) 4x^3 (x^4+1)^{-m-1} dx = 0 + 4m \int_0^\infty  \frac{x^4 dx}{(x^4+1)^{m+1}} dx
\eee

We can split the integral and arrive at

\bee
I = 4m \left( \int_0^\infty  \frac{x^4+1}{(x^4+1)^{m+1}} dx - \int_0^\infty  \frac{dx}{(x^4+1)^{m+1}} dx \right)
\eee

But now we have

\bee
I = \int_0^\infty \frac{dx}{(1+x^4)^{m}} = 4m \int_0^\infty  \frac{ dx}{(x^4+1)^{m}} - 4m \int_0^\infty  \frac{dx}{(x^4+1)^{m+1}}
\eee

and we obtain

\bee
\boxed{
\int_0^\infty  \frac{dx}{(x^4+1)^{m+1}} = \frac{4m-1}{4m} \int_0^\infty  \frac{dx}{(x^4+1)^{m}} \qed
}
\eee