\DiaryEntry{Maximum Flow, Proofs}{2020-06-09}{Algorithms}

\begin{theorem}
  Let $f$ be a flow on $G$, $G_f$ be a residual network of $G$ induced by $f$, and let $f'$ be a flow in $G_f$. Then the function $f \uparrow f'$ is a flow in $G$ with value $|f + f'| = |f| + |f'|$.
\end{theorem}

\begin{proof}
  We start with bounds for $(f \uparrow f')(u,v)$.

  \begin{align*}
    (f \uparrow f')(u,v) &= f(u,v) + f'(u,v) - f'(v,u) \\
                         &\geq f(u,v) + f'(u,v) - f(u,v) \\
                         &= f'(u,v) \\
                         &\geq 0
  \end{align*}

  In the first line we used the definition of the augmented flow; in the second line the fact that $f'(v,u) \leq f(u,v)$; i.e. the ``reverse augmenting flow'' is smaller than the ``forwad flow''.
  
  In addition, we have

  \begin{align*}
    (f \uparrow f')(u,v) &= f(u,v) + f'(u,v) - f'(v,u) \\
                         &\geq f(u,v) + f'(u,v) \\
                         &\geq f(u,v) + c_f(u,v) \\
                         &= f(u,v) + c(u,v) - f(u,v) \\
                         &= c(u,v)    
  \end{align*}

  Here we used the capacity constraint in the third line and the definition of $c_f$ in the fourth line. Summarizing, we have

  \bee
  0 \geq (f \uparrow f')(u,v) \geq c(u,v)
  \eee

  We leave the proof of shwoing that $f \uparrow f'$ is a flow in $G$ with value $|f + f'| = |f| + |f'|$.
  
\end{proof}



\begin{theorem}
  Let $f$ be a flow in a flow network $G$ and let $(S,T)$ be any cut of $G$. Then the net flow across $(S,T)$ is $|f|$; in particular it is independent of the cut.
\end{theorem}

\begin{proof}
  The flow conservation condition for any node $u \in V - \{s,t\}$ is given by

  \bee
  \sum_{v \in V} f(u,v) - \sum_{v \in V} f(v,u) = 0
  \eee

  Since the LHS is zero, we can plug it into the definition of $|f|$ as follows

  \bee
  |f| = \sum_{v \in V} f(s,v) - \sum_{v \in V} f(v,s) + \sum_{u \in S - \{s\}} \left( \sum_{v \in V} f(u,v) - \sum_{v \in V} f(v,u) \right)
  \eee

  We next expand and regroup the RHS,

  \begin{align*}
  |f| &= \sum_{v \in V} f(s,v) - \sum_{v \in V} f(v,s) + \sum_{u \in S - \{s\}} \sum_{v \in V} f(u,v) - \sum_{u \in S - \{s\}} \sum_{v \in V} f(v,u) \\
      &= \sum_{v \in V} \left( f(s,v) + \sum_{u \in S - \{s\}}f(u,v)  \right) - \sum_{v \in V} \left( f(v,s) + \sum_{u \in S - \{s\}} f(v,u)  \right) \\
      &= \sum_{v \in V} \sum_{u \in S} f(u,v) - \sum_{v \in V} \sum_{u \in S} f(v,u)
  \end{align*}

  Next we use the facts that $V = S \cup T$ and $S \cap T = 0$ to split the summations. We have

  \begin{align*}
    |f| &= \sum_{v \in S} \sum_{u \in S} f(u,v)  + \sum_{v \in T} \sum_{u \in S} f(u,v) - \sum_{v \in S} \sum_{u \in S} f(v,u) - \sum_{v \in T} \sum_{u \in S} f(v,u) \\
        &= \sum_{v \in T} \sum_{u \in S} f(u,v)  - \sum_{v \in T} \sum_{u \in S} f(v,u) + \left(\sum_{v \in S} \sum_{u \in S} f(u,v) - \sum_{v \in S} \sum_{u \in S} f(v,u) \right)\\
        &= \sum_{v \in T} \sum_{u \in S} f(u,v)  - \sum_{v \in T} \sum_{u \in S} f(v,u) \\
        &= f(S,T)
  \end{align*}

  In the third line we used the fact that the difference of the sums in brackets cancel.
\end{proof}


\begin{theorem}
  The value of any flow $f$ in a flow network $G$ is bounded above by the capacity of any cut of $G$.
\end{theorem}

\begin{proof}
  We have
  \begin{align*}
    |f| &= f(S,T) \\
        &= \sum_{u \in S} \sum_{v \in T} f(u,v) - \sum_{u \in S} \sum_{v \in T} f(v,u) \\
        &\geq \sum_{u \in S} \sum_{v \in T} f(u,v) \\
        &\geq \sum_{u \in S} \sum_{v \in T} c(u,v) \\
        &= c(S,T)
  \end{align*}
  
\end{proof}


%%% Local Variables:
%%% mode: latex
%%% TeX-master: "journal"
%%% End:
